refactor

Veir/Interpreter/Basic.lean
@@ -31,6 +31,95 @@ namespace Veir
 variable {OpInfo : Type} [HasOpInfo OpInfo]
 variable {ctx : WfIRContext OpInfo}
 
+namespace RuntimeValue
+
+@[grind <=]
+theorem Conforms.integerType :
+    Conforms runtimeValue ⟨.integerType intType, h⟩ →
+    ∃ val, runtimeValue = .int intType.bitwidth val := by
+  simp only [Conforms]
+  cases runtimeValue
+  case int bw val =>
+    simp only [int.injEq, exists_and_left]
+    intro _; subst bw
+    grind
+  all_goals grind
+
+@[grind <=]
+theorem Conforms.byteType {runtimeValue byteType h} :
+    Conforms runtimeValue ⟨.byteType byteType, h⟩ →
+    ∃ val, runtimeValue = .byte byteType.bitwidth val := by
+  simp only [Conforms]
+  cases runtimeValue
+  case byte bw val =>
+    simp only [byte.injEq, exists_and_left]
+    intro _; subst bw
+    grind
+  all_goals grind
+
+@[grind <=]
+theorem Conforms.floatType :
+    Conforms runtimeValue ⟨.floatType fltType, h⟩ →
+    ∃ val, runtimeValue = .float fltType.bitwidth val := by
+  simp only [Conforms]
+  cases runtimeValue
+  case float bw val =>
+    simp only [float.injEq, exists_and_left]
+    intro _; subst bw
+    grind
+  all_goals grind
+
+@[grind <=]
+theorem Conforms.modArithType {runtimeValue modArithType h} :
+    Conforms runtimeValue ⟨.modArithType modArithType, h⟩ →
+    ∃ val, runtimeValue = .int modArithType.modulus.type.bitwidth val := by
+  simp only [Conforms]
+  cases runtimeValue
+  case int bw val =>
+    simp only [int.injEq, exists_and_left]
+    intro _; subst bw
+    grind
+  all_goals grind
+
+@[grind <=]
+theorem Conforms.registerType :
+    Conforms runtimeValue ⟨.registerType regType, h⟩ →
+    ∃ val, runtimeValue = .reg val := by
+  simp only [Conforms]
+  cases runtimeValue <;> grind
+
+@[grind <=]
+theorem Conforms.llvmPointerType :
+    Conforms runtimeValue ⟨.llvmPointerType _, h⟩ →
+    ∃ val, runtimeValue = .addr val := by
+  simp only [Conforms]
+  cases runtimeValue <;> grind
+
+@[expose]
+def ArrayConforms (source : Array RuntimeValue) (target : Array TypeAttr) : Prop :=
+  source.size = target.size ∧ ∀ (i : Nat) (_ : i < source.size), source[i]!.Conforms target[i]!
+
+theorem ArrayConforms.take_succ_eq {source : Array RuntimeValue} {target : Array TypeAttr} :
+    source.size = target.size →
+    n < source.size →
+    (ArrayConforms (source.take (n + 1)) (target.take (n + 1)) ↔
+    (ArrayConforms (source.take n) (target.take n) ∧ (source[n]!).Conforms target[n]!)) := by
+  simp only [ArrayConforms]
+  intro hsize hn
+  constructor
+  · rintro ⟨_, h⟩
+    constructor
+    · constructor; grind
+      intro i hi
+      grind [h i]
+    · grind [h n]
+  · rintro ⟨⟨_, h⟩, hn⟩
+    constructor; grind
+    intro i hi
+    grind [h i]
+
+end RuntimeValue
+
 /--
   Memory state during interpretation.
   Set bits in the poison mask represent poison bits.
